

---

# Math 210B Notes

---

SPRING, 2026

# Contents

<b>1</b>	<b>Introduction to Rings</b>	<b>3</b>
1.1	Ring and Field Definitions . . . . .	3

# Chapter 1

## Introduction to Rings

### 1.1 Ring and Field Definitions

We move on from studying groups to studying rings and fields. First, let's compare some analogues between groups and rings.

#### Groups:

- (i) 1 operation
- (ii) Subgroups
- (iii) Normal groups  $N$
- (iv) Quotient groups  $G/N$
- (v) Morphisms of groups

#### Rings:

- (i) 2 operations
- (ii) Subrings
- (iii) Ideals  $I$
- (iv) Quotient rings  $R/I$
- (v) Morphisms of rings

We build the theory of rings and fields in a similar way to the theory of groups. An important type of ring we wish to study is the ring of polynomials with coefficients in a field. Our goal is to be able to study Galois Theory and make a connection between automorphisms of fields and their subfields.

Before we get started, consider the following example.

**Example 1.1.1.** Let  $R$  be a set with operations  $+$  and  $\times$  such that distribution holds for all elements in the set:

$$\begin{aligned}\forall a, b, c \in R \quad a \times (b + c) &= (a \times b) + (a \times c) \\ (a + b) \times c &= (a \times c) + (b \times c)\end{aligned}$$

Further assume  $+$  and  $\times$  are associative and that there exists  $1 \in R$  such that  $1 \times a = a \times 1 = a$  for all  $a \in R$ . Let  $-a$  and  $-b$  be the additive inverses of  $a, b \in R$ . Show that

$$a + b = b + a$$

**Proof.**

$$\begin{aligned}(a + b) \times (1 + 1) &= (a + b) \times 1 + (a + b) \times 1 \\ &= a \times 1 + b \times 1 + a \times 1 + b \times 1 \\ &= a + b + a + b\end{aligned}\tag{I}$$

$$\begin{aligned}(a + b) \times (1 + 1) &= a \times (1 + 1) + b \times (1 + 1) \\ &= a \times 1 + a \times 1 + b \times 1 + b \times 1 \\ &= a + a + b + b\end{aligned}\tag{II}$$

From (I) and (II), we have

$$\begin{aligned}
 a + b + a + b &= a + a + b + b \\
 \implies a + b + a + b - b &= a + a + b + b - b \\
 \implies -a + a + b + a + 0 &= -a + a + a + b + 0 \\
 \implies 0 + b + a &= 0 + a + b \\
 \implies b + a &= a + b
 \end{aligned}$$

□

This example motivates the following definition.

**Definition 1.1.1.** (Ring)

A ring is a set  $R$  together with two binary operations  $+$  (called addition) and  $\times$  (called multiplication) satisfying the following:

- (i)  $(R, +)$  is an abelian group
- (ii) Multiplication is associative  $\forall a, b, c \in R$

$$(a \times b) \times c = a \times (b \times c)$$

- (iii) Distributive laws hold  $\forall a, b, c \in R$

$$\text{Left distribution: } a \times (b + c) = (a \times b) + (a \times c)$$

$$\text{Right distribution: } (a + b) \times c = (a \times c) + (b \times c)$$

If multiplication is commutative, we call  $R$  a commutative ring. The ring  $R$  is said to have an identity denoted 1 (or contains a unity element) if

$$1 \times a = a \times 1 = a \quad \forall a \in R$$

In this case,  $R$  is called a ring with unity.

**Notation .**  $a \times b$  will be written as  $ab$ . The additive identity of  $(R, +)$  will be denoted 0. The additive inverse of an element  $a \in R$  will be denoted  $-a$ .

Notice that our definition for a ring does not require the existence of a multiplicative inverse for each element in the ring. The addition of multiplicative inverses leads to more specific types of rings, and with the addition of multiplicative commutativity, we get fields.

**Definition 1.1.2.** (Division Ring, Field)

A ring  $R$  with unity 1 (where  $1 \neq 0$ ) is called a division ring if every  $a \in R$  where  $a \neq 0$  has an element  $b \in R$  such that  $ab = ba = 1$ . That is, if all nonzero elements have a multiplicative inverse. If  $R$  is also commutative, then  $R$  is called a field.

**Example 1.1.2.** 1. Trivial rings: Given any group  $(G, *)$  if we take  $*$  as addition and define multiplication as  $ab = 0 \quad \forall a, b \in G$ , then this forms a ring.

- 2. If  $R = \{0\}$ , this is called the zero ring with multiplication and addition defined as  $0 \cdot 0 = 0$  and  $0 + 0 = 0$ . Note that this is the only ring where  $1 = 0$ . Show that if  $1 = 0$ , then  $R = \{0\}$ .

**Proof.** Let  $a \in R$ .

$$\begin{aligned}
 a \cdot 0 &= a(0 + 0) = a \cdot 0 + a \cdot 0 \\
 \implies a \cdot 0 &= a \cdot 0 + a \cdot 0 \\
 \implies 0 &= a \cdot 0 = a \cdot 1 = a
 \end{aligned}$$

□

Many theorems will state  $1 \neq 0$  instead of  $R \neq 0$ .

- 3.  $\mathbb{Z}$  with the usual multiplication and addition. Note that in  $\mathbb{Z}/\{0\}$  we do not have a group with

respect to multiplication.

4.  $\mathbb{Q}$  is a ring with the usual operations and  $\mathbb{Q}/\{0\}$  is a group with respect to multiplication, that is  $\mathbb{Q}$  is a field (multiplication in  $\mathbb{Q}$  is commutative).  $\mathbb{C}$  and  $\mathbb{R}$  are fields as well.
5.  $\mathbb{Z}/n\mathbb{Z}$  is a commutative ring with unity  $\bar{1}$  ( $\mathbb{Z}/n\mathbb{Z} = \{\bar{0}, \bar{1}, \dots, \bar{n-1}\}$ ) where the multiplication is defined  $\bar{a} \cdot \bar{b} = \overline{ab}$ .
6. The quaternions: recall the imaginary units  $i^2 = j^2 = k^2 = ijk = -1$ . Looking at the set  $\mathbb{H} = \{a + bi + cj + dk : a, b, c, d \in \mathbb{R}\}$  where addition is defined by

$$(a + bi + cj + dk) + (a' + b'i + c'j + d'k) = (a + a') + (b + b')i + (c + c')j + (d + d')k$$

and multiplication is defined by distribution

$$\begin{aligned} & (a + bi + cj + dk)(a' + b'i + c'j + d'k) \\ &= aa' - bb' - cc' - dd' + (ab' + ba' + cd' - dc')i + (a'c - bd' + ca' + db')j + (ad' + bc' - cb' + da')k \end{aligned}$$

Then  $\mathbb{H}$  forms a ring. We see that, for  $x \in \mathbb{H}$ ,

$$\begin{aligned} x\bar{x} &= (a + bi + cj + dk)(a - bi - cj - dk) = a^2 + b^2 + c^2 + d^2 \\ x^{-1} &= \frac{\bar{x}}{x\bar{x}} = \frac{a - bi - cj - dk}{a^2 + b^2 + c^2 + d^2} \end{aligned}$$

each analogous to the complex numbers. Every  $x \neq 0$  in  $\mathbb{H}$  has a multiplicative inverse. However, multiplication does not commute in all of  $\mathbb{H}$  ( $ik = -j \neq j = ki$ ), so  $\mathbb{H}$  is a division ring but not a field.

7. Let  $X$  be a nonempty set and  $A$  be any ring. The set of all mappings  $f : X \rightarrow A$  where  $(f + g)(x) = f(x) + g(x)$  and  $(fg)(x) = f(x)g(x)$  forms a ring.

Since rings add an additional operation to a group structure, we have new properties that arise from the interaction of the two operations.

**Proposition 1.1.1.** Let  $R$  be a ring.

- (i)  $0 \cdot a = a \cdot 0 = 0 \quad \forall a, b \in R$
- (ii)  $(-a)b = a(-b) = -(ab) \quad \forall a, b \in R$
- (iii)  $(-a)(-b) = ab \quad \forall a, b \in R$
- (iv) If  $R$  has identity 1, then that identity is unique and

$$-a = (-1)a \quad \forall a \in R$$

**Proof.** (i) Given  $a \in R$ , we have

$$\begin{aligned} a \cdot 0 &= a(0 + 0) = a \cdot 0 + a \cdot 0 \\ &\implies 0 = a \cdot 0 \end{aligned}$$

Similarly,

$$\begin{aligned} 0 \cdot a &= (0 + 0)a = 0 \cdot a + 0 \cdot a \\ &\implies 0 = 0 \cdot a \end{aligned}$$

- (ii) Given  $a, b \in R$ , we have

$$\begin{aligned} ab + (-a)b &= (a + -a)b \\ &= 0 \cdot b \\ &= 0 \implies -(ab) &= (-a)b \end{aligned}$$

$-(ab) = a(-b)$  is analogous.

(iii) Given  $a, b \in R$ , we have

$$\begin{aligned}
 -(ab) + (-a)(-b) &= (-a)b + (-a)(-b) \\
 &= (-a)(b + -b) \\
 &= (-a) \cdot 0 \\
 &= 0 \\
 \implies -(-ab) &= (-a)(-b) \\
 \implies ab &= (-a)(-b)
 \end{aligned}$$

(iv) Let 1 and  $e$  both be identity elements in  $R$ . Then

$$\left. \begin{array}{l} 1 \cdot e = e \\ 1 \cdot e = 1 \end{array} \right\} \implies 1 = e$$

Thus the identity element of  $R$  is unique. Let  $a \in R$  be given. We have

$$\begin{aligned}
 0 &= (1 + (-1))a \\
 &= 1 \cdot a + (-1) \cdot a \\
 &= a + (-1)a \\
 \implies -a &= (-1)a
 \end{aligned}$$

□